Just do it with Haskell.

unification/GrowTrees.hs
@@ -1,0 +1,204 @@
+{-# LANGUAGE ImportQualifiedPost, NumDecimals, RankNTypes #-}
+
+-- stack ghci --package containers --package mtl --package fgl --package graphviz --package text -- GrowTrees.hs
+
+module GrowTrees where
+
+import Control.Applicative
+import Control.Monad.State
+import Data.Char
+import Data.Foldable
+import Data.Graph.Inductive.Graph
+import Data.Graph.Inductive.Graph qualified as Graph
+import Data.Graph.Inductive.PatriciaTree
+import Data.GraphViz
+import Data.GraphViz.Attributes.Complete
+import Data.Map (Map)
+import Data.Map qualified as Map
+import Data.Maybe
+import Data.Text.Lazy (unpack)
+import Data.Tree
+import Numeric
+import Numeric.Natural
+
+instance Labellable () where
+  toLabelValue () = toLabelValue ""
+
+printPreview :: (Labellable a, Labellable b, Ord b, Graph gr) =>
+  gr a b -> String
+printPreview g = let
+  params = nonClusteredParams {
+    globalAttributes = [GraphAttrs [RankDir FromLeft]],
+    fmtNode = \ (_, l) -> [toLabel l],
+    fmtEdge = \ (_, _, l) -> [toLabel l]}
+  dg = setDirectedness graphToDot params g in
+  unpack (printDotGraph dg)
+
+treeTakeWhileWrong :: forall a. (a -> Bool) -> Tree a -> Tree a
+treeTakeWhileWrong f (Node a xs)
+  | f a = Node a (fmap (treeTakeWhileWrong f) xs)
+  | otherwise = Node a []
+
+treeTakeWhile :: forall a. (a -> Bool) -> Tree a -> Maybe (Tree a)
+treeTakeWhile f (Node a xs)
+  | f a = Just (Node a (catMaybes (fmap (treeTakeWhile f) xs)))
+  | otherwise = Nothing
+
+compactDrawTree :: Tree String -> String
+compactDrawTree = let
+  f (x : _ : xs) = x : f xs
+  f xs = xs in
+  unlines . f . lines . drawTree
+
+data Term =
+  Null Natural |
+  Un Natural Term |
+  Bin Natural Term Term
+  deriving (Eq, Ord, Show)
+
+termSize :: Term -> Natural
+termSize (Null n) = 0
+termSize (Un n x) = succ (termSize x)
+termSize (Bin n x y) = succ (termSize x + termSize y)
+
+fillHoles :: (Natural -> Term) -> Term -> [Term]
+fillHoles f (Null n) = pure (f n)
+fillHoles f (Un n x) = fmap (Un n) (fillHoles f x)
+fillHoles f (Bin n x y) =
+  liftA2 (Bin n) (pure x) (fillHoles f y) <>
+  liftA2 (Bin n) (fillHoles f x) (pure y)
+
+findHoles :: Term -> [Term -> Term]
+findHoles (Null n) = pure id
+findHoles (Un n x) = fmap (fmap (Un n)) (findHoles x)
+findHoles (Bin n x y) =
+  (liftA2 . liftA2) (Bin n) ((pure . pure) x) (findHoles y) <>
+  (liftA2 . liftA2) (Bin n) (findHoles x) ((pure . pure) y)
+
+subscript :: Char -> Char
+subscript x
+  | ord '0' <= ord x && ord x <= ord '9' =
+    chr ((ord '\8320' - ord '0') + ord x)
+  | otherwise = x
+
+showSubscript :: forall a. Integral a => a -> ShowS
+showSubscript n = showString (fmap subscript (showInt n mempty))
+
+drawTermsIxed :: Term -> ShowS
+drawTermsIxed (Null n) = showString "x" . showSubscript n
+drawTermsIxed (Un n x) = showString "(\172" . showSubscript n . showString " " .
+  drawTermsIxed x . showString ")"
+drawTermsIxed (Bin n x y) = showString "(" .
+  drawTermsIxed x . showString " \8743" . showSubscript n . showString " " .
+  drawTermsIxed y . showString ")"
+
+drawTermIxed :: Term -> String
+drawTermIxed x = drawTermsIxed x mempty
+
+drawTerms :: Term -> ShowS
+drawTerms (Null n) = showString "x"
+drawTerms (Un n x) = showString "(\172 " .
+  drawTerms x . showString ")"
+drawTerms (Bin n x y) = showString "(" .
+  drawTerms x . showString " \8743 " .
+  drawTerms y . showString ")"
+
+drawTerm :: Term -> String
+drawTerm x = drawTerms x mempty
+
+-- The path `[x, (x + x), (x + (- x)), ((- x) + (- x))]` is missing!
+growTreeWrong :: Natural -> Tree Term
+growTreeWrong 0 = pure (Null 0)
+growTreeWrong n = let n' = pred n in
+  Node (Null 0) [
+  growTreeWrong n' >>= \ x ->
+  pure (Un 0 x),
+  growTreeWrong n' >>= \ x ->
+  growTreeWrong n' >>= \ y ->
+  pure (Bin 0 x y)]
+
+-- Remove `f (Un (Null 0))` to generate associahedral trees.
+growTreeFrom :: Term -> Natural -> Tree Term
+growTreeFrom x 0 = pure x
+growTreeFrom x n = let n' = pred n in
+  Node x $
+  findHoles x >>= \ f ->
+  [f (Un 0 (Null 0)), f (Bin 0 (Null 0) (Null 0))] >>= \ y ->
+  pure (growTreeFrom y n')
+
+growTree :: Natural -> Tree Term
+growTree = growTreeFrom (Null 0)
+
+data Names = Names {
+  nameNull :: Natural,
+  nameUn :: Natural,
+  nameBin :: Natural}
+  deriving (Eq, Ord, Show)
+
+defNames :: Names
+defNames = Names {nameNull = 0, nameUn = 0, nameBin = 0}
+
+type Fresh = State Names
+
+gensymNull :: Fresh Natural
+gensymNull = state $ \ n -> (nameNull n, n {nameNull = succ (nameNull n)})
+
+gensymUn :: Fresh Natural
+gensymUn = state $ \ n -> (nameUn n, n {nameUn = succ (nameUn n)})
+
+gensymBin :: Fresh Natural
+gensymBin = state $ \ n -> (nameBin n, n {nameBin = succ (nameBin n)})
+
+labelingMachine :: Term -> Fresh Term
+labelingMachine (Null _) =
+  gensymNull >>= \ n ->
+  pure (Null n)
+labelingMachine (Un n x) =
+  gensymUn >>= \ n ->
+  labelingMachine x >>= \ a ->
+  pure (Un n a)
+labelingMachine (Bin n x y) =
+  gensymBin >>= \ n ->
+  labelingMachine x >>= \ a ->
+  labelingMachine y >>= \ b ->
+  pure (Bin n a b)
+
+label :: Term -> Term
+label x = evalState (labelingMachine x) defNames
+
+type Assign a = ((Node, Map a Node), Gr a ())
+--                ^ Node number to be assigned to the next unforeseen term.
+--                      ^ Terms seen so far with their assigned node numbers.
+--                                   ^ Graph built up to this point.
+
+cseMachine :: forall a. Ord a =>
+  Tree a -> State (Assign a) Node
+--                           ^ Node number of the root term.
+cseMachine (Node a xs) =
+  traverse cseMachine xs >>= \ ks ->
+  get >>= \ ((n, m), g) ->
+  case Map.lookup a m of
+    Nothing ->
+      put ((succ n, Map.insert a n m),
+        (insEdges (fmap (\ k -> toLEdge (n, k) ()) ks) . insNode (n, a))
+        g) >>= \ () ->
+      pure n
+    Just i -> pure i
+
+defAssign :: Assign Term
+defAssign = ((0, mempty), Graph.empty)
+
+cse :: Tree Term -> Gr Term ()
+cse x = snd (execState (cseMachine x) defAssign)
+
+main :: IO ()
+main = do
+  let n = 3
+  let t = growTree n
+  let t' = treeTakeWhile (\ x -> termSize x <= n) (growTree 1e+3)
+  if t' == Just t then
+    putStrLn "Growth matches measure!" else
+    putStrLn "Growth does not match measure!"
+  putStr . compactDrawTree . fmap (show . termSize) $ t
+  putStr . compactDrawTree . fmap drawTerm $ fmap label t
+  preview . nmap drawTerm $ cse (fmap label t)
